\section*{\underline{Aufgabe 8}}

FÃ¼r $Y \in [0,1] : Z_Y (a,b) := (a\cdot b)^{1-y}\cdot(1-(1-a)(1-b))^y$

Es gilt:

$Z_0(a,b) = (a\cdot b)^{1-0} \cdot (1-(1-a)\cdot (1-b))^0 = a\cdot b $ und

$Z_1(a,b) = (a\cdot b)^{1-1} \cdot (1-(1-a)\cdot (1-b))^1 = 1-(1-a)\cdot (1-b) $

Sein $a,b,c \in [0,1]$.

\subsection*{i) t-Norm}
1) 

$Z_0(a,1) = a\cdot1 = a$

2) 

Sei $a \leq  b$.

Dann gilt:

$Z_0(a,c) = a\cdot c = a\cdot c \leq a\cdot c + (b-a)\cdot c = b\cdot c = Z_0(b,c)$

3) 

$Z_0(a,b) = a\cdot b = b\cdot a = Z_0(b,a)$

4)

$Z_0(a,Z_0(b,c)) = a\cdot (b\cdot c) = (a\cdot b)\cdot c = Z_0(Z_0(a,b),c)$

\paragraph*{}
Aus i)1) bis i)4) folgt $Z_0$ ist t-Norm.


\subsection*{ii) s-Norm}

1) 

$Z_1(0,a) = 1-(1-0)(1-a) = 1-(1-a) = 1-1+a= a$

2) 

Sei $a \leq  b$.

$Z_0(a,c) \leq Z_0(b,c) \Leftrightarrow Z_0(a,c) - Z_0(a,b) \leq 0$

Dann gilt:

$Z_1(a,c) - Z_1(b,c) = 1 - (1-a)(1-c) - (1 - (1-b)(1-c))$

$= 1-(1-a-c+ac)- (1-(1-b-c+bc)) = a+c-ac - (b+c-bc)$

$= a-b -ac + bc = -a(c-1) + b(c-1) = \underbrace{(b-a)}_{\geq 0}\underbrace{(c-1)}_{\leq 0} \leq 0 $

3)

$Z_1(a,b) = 1-(1-a)(1-b) = 1-(1-b)(1-a) = Z_1(b,a)$

4)

$Z_1(a,Z_1(b,c)) = 1-(1-a)(1-Z_1(b,c))$

$= 1-(1-a)(1-(1-(1-b)(1-c))) = 1-(1-a)((1-b)(1-c))$

$= 1-(1-a)(1-b)(1-c) = 1 - ((1-a)(1-b))(1-c)$

$= 1 - (1-(1-(1-a)(1-b)))(1-c) = 1 - (1-Z_1(a,b))(1-c)$

$= Z_1(Z_1(a,b),c)$

\paragraph*{}

Aus ii)1) bis ii)4) folgt $Z_1$ ist s-Norm.
 


